CBPV/NormalAcc.lean
@@ -69,6 +69,20 @@ theorem StepCom.SN.letin_inv₂ {m₁ m₂} (h : StepCom.SN (.letin m₁ m₂)) 
   constructor; intro _ r
   exact ih (.letin₂ r) rfl
 
+theorem StepCom.SN.prjl_inv {m} (h : StepCom.SN (.prjl m)) : StepCom.SN m := by
+  generalize e : Com.prjl m = n at h
+  induction h generalizing m; subst e
+  case sn ih =>
+  constructor; intro _ r
+  exact ih (.prjl r) rfl
+
+theorem StepCom.SN.prjr_inv {m} (h : StepCom.SN (.prjr m)) : StepCom.SN m := by
+  generalize e : Com.prjr m = n at h
+  induction h generalizing m; subst e
+  case sn ih =>
+  constructor; intro _ r
+  exact ih (.prjr r) rfl
+
 /-*---------------
   Head expansion
 ---------------*-/
@@ -159,6 +173,26 @@ theorem StepCom.SN.case_inr' {v m n} (snv : StepVal.SN v) (snm : StepCom.SN m) (
 theorem StepCom.SN.case_inr {v m n} (snv : StepVal.SN v) (snm : StepCom.SN m) (snnv : StepCom.SN (n⦃v⦄)) : StepCom.SN (.case (.inr v) m n) :=
   .case_inr' snv snm (.antisubstitution snnv snv) snnv
 
+theorem StepCom.SN.prjl_prod {m n} (snm : StepCom.SN m) (snn : StepCom.SN n) : StepCom.SN (.prjl (.prod m n)) := by
+  induction snm generalizing n
+  induction snn
+  constructor; intro _ r; cases r
+  case a.πl h _ _ _ _ => exact .sn h
+  case a.prjl ihm _ hn ihn _ r =>
+    cases r
+    case prod₁ r => exact ihm r (.sn hn)
+    case prod₂ r => exact ihn r
+
+theorem StepCom.SN.prjr_prod {m n} (snm : StepCom.SN m) (snn : StepCom.SN n) : StepCom.SN (.prjr (.prod m n)) := by
+  induction snn generalizing m
+  induction snm
+  constructor; intro _ r; cases r
+  case a.πr h _ _ _ _ => exact .sn h
+  case a.prjr ihn _ hm ihm _ r =>
+    cases r
+    case prod₁ r => exact ihm r
+    case prod₂ r => exact ihn r (.sn hm)
+
 /-*-----------------
   Strong reduction
 -----------------*-/
@@ -172,8 +206,12 @@ inductive StepSN : Com → Com → Prop where
   | ret {v m} : StepVal.SN v → letin (ret v) m ⤳ⁿ m⦃v⦄
   | inl {v m n} : StepVal.SN v → StepCom.SN n → case (inl v) m n ⤳ⁿ m⦃v⦄
   | inr {v m n} : StepVal.SN v → StepCom.SN m → case (inr v) m n ⤳ⁿ n⦃v⦄
+  | prodl {m n} : StepCom.SN n → prjl (prod m n) ⤳ⁿ m
+  | prodr {m n} : StepCom.SN m → prjr (prod m n) ⤳ⁿ n
   | app {m n : Com} {v} : m ⤳ⁿ n → app m v ⤳ⁿ app n v
   | letin {m m' n : Com} : m ⤳ⁿ m' → letin m n ⤳ⁿ letin m' n
+  | prjl {m n} : m ⤳ⁿ n → prjl m ⤳ⁿ prjl n
+  | prjr {m n} : m ⤳ⁿ n → prjr m ⤳ⁿ prjr n
 end
 infix:40 "⤳ⁿ" => StepSN
 
@@ -220,24 +258,44 @@ theorem confluence {m n₁ n₂} (r₁ : m ⤳ᶜ n₁) (r₂ : m ⤳ⁿ n₂) :
     exact .inl ⟨_, .inr snv (h r), .refl⟩
   case inr.case₂ snv snm _ r =>
     exact .inl ⟨_, .inr snv snm, .subst _ (.once r)⟩
+  case prodl.πl => exact .inr rfl
+  case prodl.prjl snn _ r =>
+    cases r
+    case prod₁ r => exact .inl ⟨_, .prodl snn, .once r⟩
+    case prod₂ n₁ n₂ _ r =>
+    cases snn with | sn h =>
+    exact .inl ⟨n₁, .prodl (h r), .refl⟩
+  case prodr.πr => exact .inr rfl
+  case prodr.prjr snm _ r =>
+    cases r
+    case prod₂ r => exact .inl ⟨_, .prodr snm, .once r⟩
+    case prod₁ n₁ n₂ _ r =>
+    cases snm with | sn h =>
+    exact .inl ⟨n₂, .prodr (h r), .refl⟩
   case app.β r ih => cases r
   case app.app₁ snv _ ih _ r =>
-    cases ih r
-    case inl h =>
-      let ⟨_, r₁', r₂'⟩ := h
-      exact .inl ⟨_, .app r₁', .app₁ r₂'⟩
-    case inr e => subst e; exact .inr rfl
+    match ih r with
+    | .inl ⟨_, r₁', r₂'⟩ => exact .inl ⟨_, .app r₁', .app₁ r₂'⟩
+    | .inr e => subst e; exact .inr rfl
   case app.app₂ r₁' _ _ r₂' =>
     exact .inl ⟨_, .app r₁', .app₂ (.once r₂')⟩
   case letin.ζ r _ => cases r
   case letin.letin₁ ih _ r =>
-    cases ih r
-    case inl h =>
-      let ⟨_, r₁', r₂'⟩ := h
-      exact .inl ⟨_, .letin r₁', .letin₁ r₂'⟩
-    case inr e => subst e; exact .inr rfl
+    match ih r with
+    | .inl ⟨_, r₁', r₂'⟩ => exact .inl ⟨_, .letin r₁', .letin₁ r₂'⟩
+    | .inr e => subst e; exact .inr rfl
   case letin.letin₂ r₁ ih _ r₂ =>
     exact .inl ⟨_, .letin r₁, .letin₂ (.once r₂)⟩
+  case prjl.πl r _ => cases r
+  case prjl.prjl ih _ r =>
+    match ih r with
+    | .inl ⟨_, r₁', r₂'⟩ => exact .inl ⟨_, .prjl r₁', .prjl r₂'⟩
+    | .inr e => subst e; exact .inr rfl
+  case prjr.πr r _ => cases r
+  case prjr.prjr ih _ r =>
+    match ih r with
+    | .inl ⟨_, r₁', r₂'⟩ => exact .inl ⟨_, .prjr r₁', .prjr r₂'⟩
+    | .inr e => subst e; exact .inr rfl
 
 /-*-------------------------------------
   Backward closure of strong reduction
@@ -277,6 +335,27 @@ theorem closure_letin {m m' n} (r₁ : m ⤳ⁿ m') (snm : StepCom.SN m) (snn : 
     cases snlet with | sn hlet =>
     exact ihn r r₁ (.sn hn) (hlet (.letin₂ r))
 
+theorem closure_prjl {m n} (r₁ : m ⤳ⁿ n) (snn : StepCom.SN m) (snprjl : StepCom.SN (prjl n)) : StepCom.SN (prjl m) := by
+  induction snn generalizing n
+  case sn h ih =>
+  constructor; intro _ r; cases r
+  case a.πl => cases r₁
+  case a.prjl r₂ =>
+    match confluence r₂ r₁ with
+    | .inl ⟨_, r₂', r₁'⟩ => exact ih r₂ r₂' ((StepComs.prjl r₁').SN snprjl)
+    | .inr e => subst e; exact snprjl
+
+theorem closure_prjr {m n} (r₁ : m ⤳ⁿ n) (snn : StepCom.SN m) (snprjr : StepCom.SN (prjr n)) : StepCom.SN (prjr m) := by
+  induction snn generalizing n
+  case sn h ih =>
+  constructor; intro _ r; cases r
+  case a.πr => cases r₁
+  case a.prjr r₂ =>
+    match confluence r₂ r₁ with
+    | .inl ⟨_, r₂', r₁'⟩ => exact ih r₂ r₂' ((StepComs.prjr r₁').SN snprjr)
+    | .inr e => subst e; exact snprjr
+
+
 theorem StepSN.closure {m n} (r : m ⤳ⁿ n) (snn : StepCom.SN n) : StepCom.SN m := by
   induction r
   case thunk => exact .force_thunk snn
@@ -286,6 +365,10 @@ theorem StepSN.closure {m n} (r : m ⤳ⁿ n) (snn : StepCom.SN n) : StepCom.SN 
   case inr snv snm => exact .case_inr snv snm snn
   case app rn ih => exact closure_app rn (ih snn.app_inv₁) snn.app_inv₂ snn
   case letin rn ih => exact closure_letin rn (ih snn.letin_inv₁) snn.letin_inv₂ snn
+  case prodl snm => exact .prjl_prod snn snm
+  case prodr snm => exact .prjr_prod snm snn
+  case prjl r ih => exact closure_prjl r (ih snn.prjl_inv) snn
+  case prjr r ih => exact closure_prjr r (ih snn.prjr_inv) snn
 
 /-*--------------
   Neutral terms
@@ -298,6 +381,8 @@ theorem StepSN.closure {m n} (r : m ⤳ⁿ n) (snn : StepCom.SN n) : StepCom.SN 
   | app m _ => NeCom m
   | letin m _ => NeCom m
   | case v _ _ => NeVal v
+  | prjl m => NeCom m
+  | prjr m => NeCom m
   | _ => False
 
 theorem preservation :
@@ -372,3 +457,28 @@ theorem StepCom.SN.case {v m n} (nev : NeVal v) (snm : StepCom.SN m) (snn : Step
   case a.case r => cases r <;> cases nev <;> contradiction
   case a.case₁ r => exact ihm r (.sn hm)
   case a.case₂ r => exact ihn r
+
+theorem StepCom.SN.prod {m n} (snm : StepCom.SN m) (snn : StepCom.SN n) : StepCom.SN (.prod m n) := by
+  induction snm generalizing n
+  induction snn
+  case sn.sn ihm _ hm ihn =>
+  constructor; intro _ r
+  cases r
+  case a.prod₁ r => exact ihm r (.sn hm)
+  case a.prod₂ r => exact ihn r
+
+theorem StepCom.SN.prjl {m} (nem : NeCom m) (snm : StepCom.SN m) : StepCom.SN (.prjl m) := by
+  induction snm
+  case sn h ih =>
+  constructor; intro _ r
+  cases r
+  case a.πl => cases nem
+  case a.prjl r => exact ih r (r.preservation nem)
+
+theorem StepCom.SN.prjr {m} (nem : NeCom m) (snm : StepCom.SN m) : StepCom.SN (.prjr m) := by
+  induction snm
+  case sn h ih =>
+  constructor; intro _ r
+  cases r
+  case a.πr => cases nem
+  case a.prjr r => exact ih r (r.preservation nem)
